Improve tutorial

plugin/coq/Tutorial.v
@@ -1,131 +1,71 @@
-Require Import Coq.Lists.List.
+Require Import List.
 Require Import Coq.Program.Equality.
 Require Import Patcher.Patch.
 
 (*******************************************************************************)
 (*******************************************************************************)
-(* This file demonstrates using _patch registration_ on a toy formalization    *)
-(* of the simply typed lambda calculus. In particular, this development        *)
-(* simulates a scenario with the following two changes:                        *)
-(*   (a) Switching from a call-by-name to normal-order evaluation strategy     *)
+(* This file demonstrates _patch registration_ using a toy formalization of    *)
+(* the simply typed lambda calculus. In particular, this development simulates *)
+(* a scenario with the following two changes:                                  *)
+(*   (a) Switching between open and closed substitution                        *)
 (*   (b) Refactoring the conclusion of a termination theorem                   *)
+(*   (c) Using ornamentation to port lemmas from syntax with type annotations  *)
+(*       to syntax without type annotations                                    *)
+(*                                                                             *)
+(* The formalization of syntax and typing for the lambda calculus is in the    *)
+(* companion source file "Lambda.v". The specifics of that module are not      *)
+(* important for following and understanding the main tutorial. The source     *)
+(* below gives an operational semantics and interpreter implementation for the *)
+(* call-by-value evaluation strategy.                                          *)
 (*******************************************************************************)
-(*******************************************************************************)
-
-(*******************************************************************************)
-(* The formalization is in the companion source file "Lambda.v". The exact     *)
-(* details of the formalization are not important for understanding the        *)
-(* tutorial; we use this library simply to illustrate the workflow of Pumpkin  *)
-(* Patch on a concrete and realistic development project.                      *)
 (*******************************************************************************)
 
 Require Import Lambda.
 
-(*******************************************************************************)
-(* This module is our starting point. It implements a call-by-name reduction   *)
-(* semantics and proves progress and preservation w.r.t. the type system.      *)
-(*******************************************************************************)
-
-Module CallByName.
-
 (* Operational semantics *)
 Inductive step : expr -> expr -> Prop :=
-| Beta e1 t e2 : step (App (Fun t e1) e2) (e1 <- e2)
-| Left e1 e1' e2 : step e1 e1' -> step (App e1 e2) (App e1' e2).
-Notation "e1 --> e2" := (step e1 e2) (at level 40).
-
-(* Reduction sequences *)
-Inductive step_star : expr -> expr -> Prop :=
-| Refl e : step_star e e
-| Step e1 e2 e3 : step_star e1 e2 -> step e2 e3 -> step_star e1 e3.
-Notation "e1 -->* e2" := (step_star e1 e2) (at level 40).
-
-Theorem progress : forall e t, typing nil e t -> (exists e', step e e') \/ value e.
-Proof.
-  intros e t H. dependent induction H.
-  - right. constructor.
-  - left. destruct (IHtyping1 eq_refl) as [[e1' Hstep1]|Hvalue1]; clear IHtyping1.
-    + exists (App e1' e2). constructor. assumption.
-    + inversion Hvalue1 as [t0 e0 He1]. subst e1. exists (e0 <- e2). constructor.
-Qed.
-
-Lemma preservation : forall e e' t, typing nil e t -> step e e' -> typing nil e' t.
-Proof.
-  intros e e' t H. revert e'. dependent induction H; intros e' Hstep.
-  - inversion Hstep.
-  - inversion Hstep; subst. apply (subst_typing e0 t1 nil nil e2 t2); auto.
-    inversion H; subst. assumption.
-    apply TApp with (t2 := t2); try assumption. apply IHtyping1 with (e' := e1'); auto.
-Qed.
-
-Lemma progress' : forall e t, typing nil e t -> exists e', step e e' \/ value e.
-Proof.
-  intros e t Htyping. destruct (progress e t Htyping).
-  - destruct H as [e'' step]. exists e''. left. assumption.
-  - exists e. right. assumption.
-Qed.
-
-Lemma progress_patch : forall e, (exists e', step e e' \/ value e) -> (exists e', step e e') \/ value e.
-Proof.
-  intros e. destruct 1 as [e' H]. destruct H.
-  - left. exists e'. assumption.
-  - right. assumption.
-Qed.
-
-Register Patch Lemma progress_patch.
-
-Inductive cont : Set :=
-| KRet : cont
-| KApp : expr -> cont -> cont.
-
-Fixpoint rebuild (e1 : expr) (k : cont) : expr :=
-  match k with
-  | KApp e2 k => rebuild (App e1 e2) k
-  | KRet => e1
-  end.
-
-Fixpoint eval (i : nat) (e : expr) (k : cont) {struct i} : expr * cont :=
-  match i with
-  | S i =>
-    match e, k with
-    | App e1 e2, _ => eval i e1 (KApp e2 k)
-    | Fun _ e1, KApp e2 k => eval i (e1 <- e2) k
-    | _, _ => (e, k)
-    end
-  | O => (e, k)
-  end.
-
-End CallByName.
-
-(*******************************************************************************)
-(* This module is our (desired) ending point. It implements a call-by-value    *)
-(* reduction semantics and proves progress and preservation w.r.t. the type    *)
-(* system. In the next step, we'll show how to generate the update lemmas      *)
-(* from the previous module by patching.                                       *)
-(*******************************************************************************)
-
-Module CallByValue.
-
-(* Operational semantics *)
-Inductive step : expr -> expr -> Prop :=
-| Beta e1 t e2 :
+| BetaAx e1 t e2 :
     value e2 ->
     step (App (Fun t e1) e2) (e1 <- e2)
-| Left e1 e1' e2 :
+| LeftCx e1 e1' e2 :
     step e1 e1' ->
     step (App e1 e2) (App e1' e2)
-| Right e1 e2 e2' :
+| RightCx e1 e2 e2' :
     value e1 -> step e2 e2' ->
     step (App e1 e2) (App e1 e2').
 Notation "e1 --> e2" := (step e1 e2) (at level 40).
 
-(* Reduction sequences *)
-Inductive step_star : expr -> expr -> Prop :=
-| Refl e : step_star e e
-| Step e1 e2 e3 : step_star e1 e2 -> step e2 e3 -> step_star e1 e3.
-Notation "e1 -->* e2" := (step_star e1 e2) (at level 40).
+(* Reduction semantics: reflexive, transitive closure of operational semantics *)
+Inductive reduces : expr -> expr -> Prop :=
+| Refl e : reduces e e
+| Step e1 e2 e3 : reduces e1 e2 -> step e2 e3 -> reduces e1 e3.
+Notation "e1 ==> e2" := (reduces e1 e2) (at level 40).
 
-Theorem progress : forall e t, typing nil e t -> (exists e', step e e') \/ value e.
+(* Reduction semantics closed under left-stepping *)
+Lemma reduces_left e1 e1' e2 :
+  e1 ==> e1' -> App e1 e2 ==> App e1' e2.
+Proof.
+  intros H. induction H as [e1|e1 e1'' e1' Hreduces1 IH Hstep1]; try constructor.
+  eapply Step. exact IH. apply LeftCx. assumption.
+Qed.
+
+(* Reduction semantics closed under right-stepping *)
+Lemma reduces_right e1 e2 e2' :
+  value e1 -> e2 ==> e2' -> App e1 e2 ==> App e1 e2'.
+Proof.
+  intros Hval H. induction H as [e2|e2 e2'' e2' Hreduces1 IH Hstep2]; try constructor.
+  eapply Step. exact IH. apply RightCx; assumption.
+Qed.
+
+(* Reduction semantics transitive *)
+Lemma reduces_trans e1 e2 e3 :
+  e1 ==> e2 -> e2 ==> e3 -> e1 ==> e3.
+Proof.
+  intros Hreduces1 Hreduces2. induction Hreduces2; try assumption.
+  eapply Step; (try apply IHHreduces2); assumption.
+Qed.
+
+Lemma progress : forall e t, typing nil e t -> (exists e', e --> e') \/ value e.
 Proof.
   intros e t H. dependent induction H.
   - right. constructor.
@@ -137,30 +77,46 @@ Proof.
         exists (e0 <- e2). constructor; assumption.
 Qed.
 
-Theorem preservation : forall e e' t, typing nil e t -> step e e' -> typing nil e' t.
+Lemma preservation : forall e e' t, typing nil e t -> e --> e' -> typing nil e' t.
 Proof.
   intros e e' t H. revert e'. dependent induction H; intros e' Hstep.
   - inversion Hstep.
-  - inversion Hstep; subst; try (apply TApp with (t2 := t2); auto).
+  - inversion Hstep; subst; try (apply AppTy with (t2 := t2); auto).
     inversion H; subst. apply (subst_typing e0 t1 nil nil e2 t2); auto.
 Qed.
 
-Inductive cont : Set :=
-| KRet : cont
-| KApp : expr -> cont -> cont
-| KArg : expr -> cont -> cont.
-
-Fixpoint eval (i : nat) (e : expr) (k : cont) {struct i} : expr * cont :=
-  match i with
-  | S i =>
-    match e, k with
-    | App e1 e2, _ => eval i e2 (KArg e1 k)
-    | Fun _ e1, KApp e2 k => eval i (e1 <- e2) k
-    | e2, KArg e1 k => eval i e1 (KApp e2 k)
-    | _, _ => (e, k)
+Fixpoint eval (n : nat) (e : expr) {struct n} : expr :=
+  match n, e with
+  | S n, App e1 e2 =>
+    match eval n e1, eval n e2 with
+    | Fun t1 e1', Fun t2 e2' =>
+      eval n (e1' <- Fun t2 e2')
+    | Fun t1 e1', e2' =>
+      App (Fun t1 e1') e2'
+    | e1', _ => App e1' e2
     end
-  | O => (e, k)
+  | _, _ => e
   end.
 
-End CallByValue.
-
+(* Evaluation is sound w.r.t. the reduction semantics *)
+Theorem eval_ok e e' n : eval n e = e' -> e ==> e'.
+Proof.
+  revert e e'.
+  induction n as [|n IH]; simpl; intros e e' E; try (rewrite <- E; constructor).
+  (* Case analysis on the expression *)
+  destruct e as [i|e1|e1 e2]; try (rewrite <- E; constructor).
+  (* Evaluation of an operator expression is sound *)
+  destruct (eval n e1) as [i1|e11|e11 e12] eqn:He1; apply IH in He1;
+    eapply reduces_trans;
+    try (eapply reduces_left; exact He1);
+    try (rewrite <- E; apply Refl).
+  (* Evaluation of an operand expression is sound *)
+  destruct (eval n e2) as [i2|e21|e21 e22] eqn:He2; apply IH in He2;
+    eapply reduces_trans;
+    try (eapply reduces_right; [constructor|exact He2]);
+    try (rewrite <- E; apply Refl).
+  (* Evaluation of a beta-redex is sound *)
+  apply IH in E. eapply reduces_trans.
+  - eapply Step. apply Refl. constructor. constructor.
+  - assumption.
+Qed.
